src/SDK/MessageHeader/Utils.dfy
@@ -101,4 +101,33 @@ module MessageHeader.Utils {
   {
     SortedKVPairsUpTo(a, |a|)
   }
+
+  method InsertNewEntry(kvPairs: seq<(seq<uint8>, seq<uint8>)>, key: seq<uint8>, value: seq<uint8>)
+      returns (res: Option<seq<(seq<uint8>, seq<uint8>)>>, ghost insertionPoint: nat)
+    requires SortedKVPairs(kvPairs)
+    ensures match res
+    case None =>
+      exists i :: 0 <= i < |kvPairs| && kvPairs[i].0 == key  // key already exists
+    case Some(kvPairs') =>
+      && insertionPoint <= |kvPairs|
+      && kvPairs' == kvPairs[..insertionPoint] + [(key, value)] + kvPairs[insertionPoint..]
+      && SortedKVPairs(kvPairs')
+  {
+    var n := |kvPairs|;
+    while 0 < n && LexCmpSeqs(key, kvPairs[n - 1].0, UInt8Less)
+      invariant 0 <= n <= |kvPairs|
+      invariant forall i :: n <= i < |kvPairs| ==> LexCmpSeqs(key, kvPairs[i].0, UInt8Less)
+    {
+      n := n - 1;
+    }
+    if 0 < n && kvPairs[n - 1].0 == key {
+      return None, n;
+    } else {
+      var kvPairs' := kvPairs[..n] + [(key, value)] + kvPairs[n..];
+      if 0 < n {
+        LexPreservesTrichotomy(kvPairs'[n - 1].0, kvPairs'[n].0, UInt8Less);
+      }
+      return Some(kvPairs'), n;
+    }
+  }
 }
